composed_vlsm_projections.v
@@ -1,0 +1,298 @@
+From Casper
+Require Import vlsm composed_vlsm.
+
+Definition vlsm_projection_initial_state_prop
+  {message : Type}
+  `{CV : composed_vlsm_class message}
+  (i : index)
+  (is : istate i)
+  : Prop
+  :=
+  exists s : initial_state, istate_proj i (proj1_sig s) = proj1_sig is.
+
+Definition vlsm_projection_initial_state
+  {message : Type}
+  `{CV : composed_vlsm_class message}
+  (i : index)
+  :=
+  { s : istate i | vlsm_projection_initial_state_prop i s }.
+
+Lemma vlsm_projection_protocol_state_inhabited
+  {message : Type}
+  `{CV : composed_vlsm_class message}
+  (i : index)
+  : inhabited (vlsm_projection_initial_state i).
+Proof.
+  destruct protocol_state_inhabited as [s].
+  remember (proj_istate (proj1_sig s) i) as iis.
+  assert (Hiis : vlsm_projection_initial_state_prop i iis)
+    by (exists s; subst; reflexivity).
+  constructor. exact (exist _ iis Hiis).
+Qed.
+
+Definition lift_proto_message
+  {message : Type}
+  `{CV : composed_vlsm_class message}
+  (i : index)
+  (m : {x : message | iproto_message_prop i x})
+  : proto_message
+  :=
+  let m0 := proj1_sig m in
+  let Hcm := iproto_message_consistent i m0 (proj2_sig m) in
+  (exist _ m0 Hcm).
+
+Definition vlsm_projection_initial_message_prop
+  {message : Type}
+  `{CV : composed_vlsm_class message}
+  (i : index)
+  (m : {x : message | iproto_message_prop i x})
+  : Prop
+  :=
+  protocol_message_prop (lift_proto_message i m).
+
+Definition vlsm_projection_valid
+  {message : Type}
+  `{CV : composed_vlsm_class message}
+  (i : index)
+  (il : ilabel_type i)
+  (isom : istate i * option {m : message | iproto_message_prop i m})
+  : Prop
+  :=
+  let l := proj1_sig il in
+  let (is, oim) := isom in
+  let om := option_map (lift_proto_message i) oim in
+  exists s : state, istate_proj i s = proj1_sig is /\ valid l (s, om)
+  .
+
+
+(* 
+message : Type
+H : VLSM message
+CV : composed_vlsm_class message
+i : index
+l : label
+Hl : ilabel l = i
+is : iproto_state i
+s : state
+His : istate_proj i s = is
+iom : option {m : message | iproto_message_prop i m}
+om : option proto_message
+Heqom : om = option_map (lift_proto_message i) iom
+s' : state
+m' : proto_message
+Heqt : (s', Some m') = transition l (s, om)
+Hmsg : iproto_message_prop i (proj1_sig m')
+*)
+Definition transitioning_projection
+  {message : Type}
+  `{CV : composed_vlsm_class message}
+  (i : index)
+  (il : ilabel_type i)
+  (isom isom' : istate i * option {m : message | iproto_message_prop i m})
+  :=
+  exists (s s' : state),
+    proj_istate s i = fst isom /\
+    proj_istate s' i = fst isom' /\
+    transition (proj1_sig il) (s, (option_map (lift_proto_message i) (snd isom))) = (s', (option_map (lift_proto_message i) (snd isom')))
+  .
+
+Lemma vlsm_projection_transition_existance
+  {message : Type}
+  `{CV : composed_vlsm_class message}
+  (i : index)
+  (il : ilabel_type i)
+  (isom : istate i * option {m : message | iproto_message_prop i m})
+  : exists isom' : istate i * option {m : message | iproto_message_prop i m}, 
+      transitioning_projection i il isom isom'.
+Proof.
+  destruct isom as [is iom].
+  destruct il as [l Hl].
+  destruct is as [is [s His]].
+  remember (option_map (lift_proto_message i) iom) as om.
+
+  specialize transition_projection_type_preservation; intros Hmsg.
+  specialize (Hmsg s om l i Hl).
+
+  remember (transition l (s, om)) as t.
+  destruct t as [s' om'].
+
+  destruct om' as [m'|]; simpl in Hmsg.
+  - exists (proj_istate s' i, Some (exist _ (proj1_sig m') Hmsg)).
+    exists s. exists s'. rewrite <- His.
+    simpl. repeat split; try reflexivity.  rewrite <- Heqom. rewrite <- Heqt.
+    apply f_equal. apply f_equal.
+    unfold lift_proto_message; simpl.
+    apply exist_eq. reflexivity.
+  - exists (proj_istate s' i, None).
+    exists s. exists s'. rewrite <- His. 
+    simpl. repeat split; try reflexivity.
+    rewrite <- Heqom. symmetry.  assumption.
+Qed.
+
+Require Import Coq.Logic.ClassicalEpsilon.
+
+Definition vlsm_projection_transition
+  {message : Type}
+  `{CV : composed_vlsm_class message}
+  (i : index)
+  (il : ilabel_type i)
+  (isom : istate i * option {m : message | iproto_message_prop i m})
+  : istate i * option {m : message | iproto_message_prop i m}
+  :=
+  (proj1_sig
+    (constructive_indefinite_description
+      (transitioning_projection i il isom)
+      (vlsm_projection_transition_existance i il isom)
+    )
+  ).
+
+Lemma vlsm_projection_transition_irrelevance
+  {message : Type}
+  `{CV : composed_vlsm_class message}
+  (i : index)
+  (il : ilabel_type i)
+  (s1 s2 : istate i)
+  (Heqi : proj1_sig s1 = proj1_sig s2)
+  (om : option {m : message | iproto_message_prop i m})
+  : vlsm_projection_transition i il (s1, om) = vlsm_projection_transition i il (s2, om).
+Proof.
+  assert (Heq : s1 = s2 ).
+  { destruct s1 as [s1 Hs1]. destruct s2 as [s2 Hs2]. apply exist_eq. assumption. }
+  subst. reflexivity.
+Qed.
+
+Definition vlsm_projection
+  {message : Type}
+  `{CV : composed_vlsm_class message}
+  (i : index)
+  : VLSM (message : Type)
+  :=
+  {|  state := istate i
+  ;   label := ilabel_type i
+  ;   proto_message_prop := iproto_message_prop i
+  ;   proto_message_decidable := iproto_message_decidable i
+  ;   initial_state_prop := vlsm_projection_initial_state_prop i
+  ;   initial_message_prop := vlsm_projection_initial_message_prop i
+  ;   transition := vlsm_projection_transition i
+  ;   protocol_state_inhabited := vlsm_projection_protocol_state_inhabited i
+  ;   message_inhabited := iproto_message_inhabited i
+  ;   label_inhabited := ilabel_type_inhabited i
+  ;   valid := vlsm_projection_valid i
+  |}.
+
+
+Lemma protocol_state_projection
+  {message : Type}
+  {V : VLSM message}
+  `{CV : @composed_vlsm_class message V}
+  : forall (i : index) (s :  protocol_state),
+  @protocol_state_prop _ (vlsm_projection i) (proj_istate (proj1_sig s) i).
+Proof.
+  intros i [s Hps]. simpl. induction Hps as [is | s s'' l om' Hps Hp Hv Ht| s s'' l m om' Hps Hp Hpm Hv Ht].
+  - apply protocol_state_prop_iff. left. 
+    remember (proj_istate (proj1_sig is) i) as iis.
+    unfold initial_state.
+    unfold initial_state_prop; simpl. unfold vlsm_projection_initial_state_prop.
+    assert (His : exists s0 : initial_state, istate_proj i (proj1_sig s0) = proj1_sig iis)
+      by (exists is; subst; reflexivity).
+    exists (exist _ iis His); reflexivity.
+  - remember None as om. 
+(* 
+    assert (Hps' : protocol_state_prop (fst (transition l (s, om)))).
+    { apply protocol_state_prop_iff. right. exists (exist _ s Hps). exists l. exists None. 
+      unfold protocol_valid; unfold protocol_transition; simpl. split; subst; try assumption; reflexivity. }
+ *)
+    remember (ilabel l) as j.
+    destruct (index_eq_dec i j); subst.
+    + apply protocol_state_prop_iff. right.
+      exists (exist _ (proj_istate s (ilabel l)) Hp).
+      remember (ilabel l) as j. symmetry in Heqj.
+      exists (exist _ l Heqj).
+      exists None. split.
+      * unfold protocol_valid. simpl. exists s. split; try reflexivity. assumption.
+      * simpl. unfold vlsm_projection_transition.
+        remember
+          (@constructive_indefinite_description
+           (prod (@istate message V CV j)
+              (option (@sig message (fun m : message => @iproto_message_prop message V CV j m))))
+           (@transitioning_projection message V CV j
+              (@exist (@label message V)
+                 (fun l0 : @label message V =>
+                  @eq (@index message V CV) (@ilabel message V CV l0) j) l Heqj)
+              (@pair (@istate message V CV j)
+                 (option (@proto_message message (@vlsm_projection message V CV j)))
+                 (@proj_istate message V CV s j)
+                 (@None (@proto_message message (@vlsm_projection message V CV j)))))
+           (@vlsm_projection_transition_existance message V CV j
+              (@exist (@label message V)
+                 (fun l0 : @label message V =>
+                  @eq (@index message V CV) (@ilabel message V CV l0) j) l Heqj)
+              (@pair (@istate message V CV j)
+                 (option (@proto_message message (@vlsm_projection message V CV j)))
+                 (@proj_istate message V CV s j)
+                 (@None (@proto_message message (@vlsm_projection message V CV j)))))
+          ) as sjom'.
+      clear Heqsjom'.
+      destruct sjom' as [sjom' Hsjom'].
+      rename om' into om''.
+      destruct sjom' as [sj' om'].
+      destruct Hsjom' as [s0 [s0' Hsjom']]. simpl in Hsjom'.
+      destruct Hsjom' as [Heqs0 [Heqs0' Ht0]]. simpl.
+      specialize transition_projection_consistency; intros Hpc.
+      apply proj_istate_eq in Heqs0.
+      specialize (Hpc s0 s None l j Heqs0 Heqj).
+      rewrite Ht in Hpc. simpl in Hpc. destruct Hpc as [Hmsg Hst].
+      apply proj_istate_eq in Hst. rewrite <- Hst. 
+      rewrite Ht0. simpl. assumption.
+    + specialize (transition_projection_state_preservation s None l i); intros Htp.
+      assert (ni : ilabel l <> i) by (intro; subst; contradiction).
+      specialize (Htp ni). rewrite Ht in Htp. simpl in Htp.
+      apply proj_istate_eq in Htp.
+      rewrite Htp. assumption.
+  - remember (Some m) as om.
+    remember (ilabel l) as j.
+    destruct (index_eq_dec i j); subst.
+(* 
+    + apply protocol_state_prop_iff. right.
+      remember (ilabel l) as j. exists (exist _ (proj_istate s j) Hp).
+      symmetry in Heqj.
+      exists (exist _ l Heqj).
+      
+      exists (Some (lift_proto_message j (exist _ m Hpm))). split.
+      * unfold protocol_valid. simpl. exists s. split; try reflexivity. assumption.
+      * simpl. unfold vlsm_projection_transition.
+        remember
+          (@constructive_indefinite_description
+           (prod (@istate message V CV j)
+              (option (@sig message (fun m : message => @iproto_message_prop message V CV j m))))
+           (@transitioning_projection message V CV j
+              (@exist (@label message V)
+                 (fun l0 : @label message V =>
+                  @eq (@index message V CV) (@ilabel message V CV l0) j) l Heqj)
+              (@pair (@istate message V CV j)
+                 (option (@proto_message message (@vlsm_projection message V CV j)))
+                 (@proj_istate message V CV s j)
+                 (@None (@proto_message message (@vlsm_projection message V CV j)))))
+           (@vlsm_projection_transition_existance message V CV j
+              (@exist (@label message V)
+                 (fun l0 : @label message V =>
+                  @eq (@index message V CV) (@ilabel message V CV l0) j) l Heqj)
+              (@pair (@istate message V CV j)
+                 (option (@proto_message message (@vlsm_projection message V CV j)))
+                 (@proj_istate message V CV s j)
+                 (@None (@proto_message message (@vlsm_projection message V CV j)))))
+          ) as sjom'.
+      clear Heqsjom'.
+      destruct sjom' as [sjom' Hsjom'].
+      rename om' into om''.
+      destruct sjom' as [sj' om'].
+      destruct Hsjom' as [s0 [s0' Hsjom']]. simpl in Hsjom'.
+      destruct Hsjom' as [Heqs0 [Heqs0' Ht0]]. simpl.
+      specialize transition_projection_consistency; intros Hpc.
+      apply proj_istate_eq in Heqs0.
+      specialize (Hpc s0 s None l j Heqs0 Heqj).
+      rewrite Ht in Hpc. simpl in Hpc. destruct Hpc as [Hmsg Hst].
+      apply proj_istate_eq in Hst. rewrite <- Hst. 
+      rewrite Ht0. simpl. assumption.
+ *)
+Admitted.
